Qed! (Kinda)

theories/abs_functional_metatheory.v
@@ -20,15 +20,13 @@ Hypothesis (vars_well_typed: forall (x_:x) (G0: G) T0,
              Map.find x_ G0 = Some T0 ->
              exists T_, T0 = ctxv_T T_).
 
-Notation "G ⊢ e : T" := (typ_e G e T) (at level 5).
-Notation "G F⊢ F" := (typ_F G F) (at level 5).
-(* Notation "Fs , s ⊢ e ⇝ s' ⊢ e'" := (red_e Fs s e s' e') (at level 10). *)
-
 Definition subG (G1 G2 : G) : Prop :=
-  forall (key : string) (elt : ctxv), 
+  forall (key : string) (elt : ctxv),
     Map.find key G1 = Some elt ->
     Map.find key G2 = Some elt.
 
+Notation "G ⊢ e : T" := (typ_e G e T) (at level 5).
+Notation "G F⊢ F" := (typ_F G F) (at level 5).
 Notation "G1 ⊆ G2" := (subG G1 G2) (at level 5).
 
 Lemma subG_refl: forall G0,
@@ -86,22 +84,6 @@ Definition G_vdash_s (G5 : G) (s5 : s) :=
   Map.find x5 s5 = Some t5 /\ typ_e G5 (e_t t5) T5.
 
 Notation "G1 G⊢ s1" := (G_vdash_s G1 s1) (at level 5).
-
-(* how is this not in MapFacts? *)
-Lemma map_neq_none_is_some{elt:Type}: forall m x,
-  Map.find x m <> None ->
-  exists y, Map.find (elt:=elt) x m = Some y.
-Proof.
-  intros.
-  destruct (MapFacts.In_dec m x).
-  - inv i.
-    exists x0.
-    apply Map.find_1.
-    apply H0.
-  - apply MapFacts.not_find_in_iff in n.
-    rewrite n in H.
-    contradiction.
-Qed.
 
 Lemma fresh_subG: forall G0 s0 (sub_list: list (T*x*t*x)),
   G_vdash_s G0 s0 ->
@@ -216,48 +198,9 @@ Proof.
       apply H2.
 Qed.
 
-(* some slightly ad-hoc equalities *)
-Lemma subst_fst_commute: forall x0 x1 e_T_list,
-  map (fun x : e * T => let (e_, _) := let '(e_, T_) := x in (e_var_subst_one e_ x0 x1, T_) in e_) e_T_list =
-  (fix e_list_subst_one (es : list e) (x_ y_ : x) {struct es} : list e :=
-     match es with
-     | [] => fun _ _ : x => []
-     | e :: l => fun x_0 y_0 : x => e_var_subst_one e x_0 y_0 :: e_list_subst_one l x_0 y_0
-     end x_ y_) (map (fun pat_ : e * T => let (e_, _) := pat_ in e_) e_T_list) x0 x1.
-Proof.
-  induction e_T_list; auto.
-  destruct a.
-  simpl.
-  rewrite <- IHe_T_list.
-  reflexivity.
-Qed.
-
-Lemma subst_snd_commutes: forall x0 s e_T_list,
-  map (fun pat_ : e * T => let (_, T_) := pat_ in T_)
-    (map (fun pat_ : e * T => let (e_, T_) := pat_ in (e_var_subst_one e_ x0 s, T_)) e_T_list) =
-    map (fun pat_ : e * T => let (_, T_) := pat_ in T_) e_T_list.
-Proof.
-  intros.
-  induction e_T_list; auto.
-  destruct a;cbn in *.
-  now rewrite IHe_T_list.
-Qed.
-
-Lemma fold_map_reshuffle: forall (l: list (T*x*t*x)) G0,
-  (fold_right (fun (ax : x * T) (G' : G) => Map.add (fst ax) (ctxv_T (snd ax)) G') G0
-     (map (fun pat_ : T * x => let (T_, x_) := pat_ in (x_, T_)) (map (fun '(T_0, x_, _, _) => (T_0, x_)) l)))
-  = (fold_right (fun '(T1, x_, _, _) (G' : G) => Map.add x_ (ctxv_T T1) G') G0 l).
-Proof.
-  induction l;intros;auto.
-  destruct a as (((?T_ & ?x_) & ?t_) & ?y).
-  simpl.
-  rewrite IHl.
-  reflexivity.
-Qed.
-
 (* this is 9.3.8 from Types and Programming Languages *)
 (* it has not yet proven useful *)
-Lemma subst_lemma_one: forall (x0 x1:x) G0 e0 T0 T1,
+Lemma subst_lemma_one_alt: forall (x0 x1:x) G0 e0 T0 T1,
   typ_e (Map.add x0 (ctxv_T T1) G0) e0 T0 ->
   typ_e G0 (e_var x1) T1 ->
   typ_e G0 (e_var_subst_one e0 x0 x1) T0.
@@ -324,205 +267,6 @@ Proof.
     + eapply H; eauto.
     + eapply H0; eauto.
 Qed.
-
-Lemma subst_term: forall t sub,
-  e_var_subst (e_t t) sub = (e_t t).
-Proof.
-  induction sub.
-  - trivial.
-  - destruct a.
-    simpl.
-    rewrite IHsub.
-    now simp e_var_subst_one.
-Qed.
-
-Definition replace_var (x0:x) (sub:list(x*x)) :=
- fold_right (fun '(x_, y_) x0 => if (eq_x x0 x_) then y_ else x0) x0 sub.
-
-Lemma subst_var: forall x0 sub,
-  e_var_subst (e_var x0) sub = e_var (replace_var x0 sub).
-Proof.
-  induction sub.
-  - trivial.
-  - destruct a; simpl.
-    rewrite IHsub.
-    simp e_var_subst_one.
-    destruct (eq_x (replace_var x0 sub)); subst; eauto.
-Qed.
-
-Lemma e_list_subst_map: forall x0 y0 e_list,
-  e_list_subst_one e_list x0 y0 = map (fun e_ => e_var_subst_one e_ x0 y0) e_list.
-Proof.
-  induction e_list; [easy|];
-  destruct a;
-    simpl;
-    now rewrite IHe_list.
-Qed.
-
-Lemma subst_fn: forall fn0 sub e_list,
-  e_var_subst (e_fn_call fn0 e_list) sub = (e_fn_call fn0 (map (fun e' => e_var_subst e' sub) e_list)).
-Proof.
-  induction sub; intros.
-  - simpl.
-    now rewrite map_id.
-  - destruct a.
-    simpl.
-    rewrite IHsub.
-    simp e_var_subst_one.
-    now rewrite e_list_subst_map, map_map.
-Qed.
-
-Lemma e_list_subst: forall el x0 y0,
-  e_list_subst_one el x0 y0 = map (fun e => e_var_subst_one e x0 y0) el.
-Proof.
-  induction el; intros.
-  - trivial.
-  - simpl.
-    now rewrite IHel.
-Qed.
-
-Lemma e_list_fresh: forall e0 ys el,
-  fresh_vars_el ys el ->
-  In e0 el ->
-  fresh_vars_e ys e0.
-Proof.
-  induction el.
-  - easy.
-  - simpl; intros.
-    destruct H0; subst.
-    + now destruct H.
-    + destruct H.
-      apply IHel; eauto.
-Qed.
-
-Lemma fresh_vars_first: forall e0 y ys,
-  fresh_vars_e (y::ys) e0 -> fresh_vars_e [y] e0.
-Proof.
-  induction e0 using e_ott_ind
-    with (P_list_e := fun e_list =>
-                        forall e0 y ys,
-                        In e0 e_list ->
-                        fresh_vars_e (y::ys) e0 -> fresh_vars_e [y] e0);
-     intros; try easy.
-  - simp fresh_vars_e in *.
-    intro.
-    inv H0.
-    + apply H.
-    now left.
-    + inv H1.
-  - simp fresh_vars_e in *.
-    induction e_list.
-    + easy.
-    + inv H.
-      split.
-      * eapply IHe0; eauto.
-        now left.
-      * eapply IHe_list; eauto.
-        intros; eapply IHe0; eauto.
-        now right.
-  - inv H.
-    + eapply IHe0; eauto.
-    + eapply IHe1; eauto.
-Qed.
-
-Lemma fresh_monotone_e: forall e0 y ys,
-  fresh_vars_e (y::ys) e0 -> fresh_vars_e ys e0.
-Proof.
-  induction e0 using e_ott_ind
-    with (P_list_e := fun e_list =>
-                        forall e0 y ys,
-                        In e0 e_list ->
-                        fresh_vars_e (y::ys) e0 -> fresh_vars_e ys e0);
-     intros; try easy.
-  - simp fresh_vars_e in *.
-    intro.
-    apply H.
-    right.
-    assumption.
-  - simp fresh_vars_e in *.
-    induction e_list.
-    + easy.
-    + inv H.
-      split.
-      * eapply IHe0; eauto.
-        now left.
-      * apply IHe_list; eauto.
-        intros; eapply IHe0; eauto.
-        now right.
-  - inv H.
-    + eapply IHe0; eauto.
-    + eapply IHe1; eauto.
-Qed.
-
-Lemma map_add_comm{E:Type}: forall m key key' elt elt',
-  key <> key' -> Map.Equal (Map.add (elt:=E) key elt (Map.add key' elt' m)) (Map.add key' elt' (Map.add key elt m)).
-Proof.
-  intros.
-  intro.
-  destruct (Map.find y m) eqn:?.
-  - destruct (eq_x y key), (eq_x y key'); subst;
-      erewrite 2 Map.find_1; eauto;
-      (* this should just be "eauto with map", but I can't seem to import the hint database *)
-      try (apply Map.add_2; eauto; now apply Map.add_1);
-      try (now apply Map.add_1; eauto);
-      try (repeat (apply Map.add_2; eauto); now apply Map.find_2; eauto).
-  - destruct (eq_x y key), (eq_x y key'); subst.
-    + contradiction.
-    + erewrite 2 Map.find_1; eauto.
-      * apply Map.add_2; eauto.
-        now apply Map.add_1.
-      * now apply Map.add_1.
-    + erewrite 2 Map.find_1; eauto.
-      * now apply Map.add_1.
-      * apply Map.add_2; eauto.
-        now apply Map.add_1.
-
-    (* there has to be a cleaner way to do this case?? *)
-    + replace (Map.find (elt:=E) y (Map.add key elt (Map.add key' elt' m))) with (@None E).
-      replace (Map.find (elt:=E) y (Map.add key' elt' (Map.add key elt m))) with (@None E).
-      reflexivity.
-      * symmetry.
-        apply MapFacts.not_find_in_iff in Heqo.
-        apply MapFacts.not_find_in_iff.
-        intro.
-        inv H0.
-        apply Heqo.
-        exists x.
-        eapply Map.add_3; eauto.
-        eapply Map.add_3; eauto.
-      * symmetry.
-        apply MapFacts.not_find_in_iff in Heqo.
-        apply MapFacts.not_find_in_iff.
-        intro.
-        inv H0.
-        apply Heqo.
-        exists x.
-        eapply Map.add_3; eauto.
-        eapply Map.add_3; eauto.
-Qed.
-
-Lemma fold_not_in: forall G0 y (T_x_t_y_list: list (T*x*t*x)),
-  ~ Map.In y G0 ->
-  ~ In y (map (fun '(_, _, _, y') => y') T_x_t_y_list) ->
-  ~ Map.In y (fold_right (fun '(T_, _, _, y) (G0 : G) => Map.add y (ctxv_T T_) G0) G0 T_x_t_y_list).
-Proof.
-  induction T_x_t_y_list as [ | (((?T_, ?x_), ?t_), ?y) T_x_t_y_list IH ]; [easy|].
-  simpl; intros ? ? ?.
-  destruct (eq_x y y0); subst.
-  - apply H0.
-    now left.
-  - apply MapFacts.add_in_iff in H1.
-    inv H1.
-    + apply H0.
-      now left.
-    + apply IH; eauto.
-Qed.
-
-Lemma fold_add_comm: forall G0 y T_ (upd: list (T*x*t*x)),
-  ~ In y (map (fun '(_,_,_, y) => y) upd) ->
-  Map.add y (ctxv_T T_) (fold_right (fun '(T_,_,_, y) G0 => Map.add y (ctxv_T T_) G0) G0 upd)
-  = (fold_right (fun '(T_,_,_, y) G0 => Map.add y (ctxv_T T_) G0) (Map.add y (ctxv_T T_) G0) upd).
-Admitted.
 
 Lemma same_type_sub: forall (sub_list: list (x*x)) G0 e0 T0,
     typ_e G0 e0 T0 ->
@@ -595,7 +339,7 @@ Proof.
 
 Qed.
 
-Lemma subst_lemma_one_alt: forall G0 x0 y0 e0 Ai A,
+Lemma subst_lemma_one: forall G0 x0 y0 e0 Ai A,
   typ_e (Map.add x0 Ai G0) e0 A ->
   fresh_vars_e [y0] e0 ->
   typ_e (Map.add y0 Ai G0) (e_var_subst_one e0 x0 y0) A.
@@ -681,52 +425,79 @@ Proof.
     - destruct H1; subst.
       + apply H; eauto.
       + apply H0; eauto.
-
   }
 Qed.
 
-Lemma fresh_subst_NoDup: forall e0 y sub,
-  fresh_vars_e [y] e0 ->
-  ~ In y (map (fun '(_, y) => y) sub) ->
-  fresh_vars_e [y] (e_var_subst e0 sub).
-Admitted.
-
-(* pipe dream: might need some stronger assumptions*)
 Lemma subst_lemma: forall (T_x_t_y_list:list (T*x*t*x)) G0 e0 A,
   typ_e (fold_right (fun '(Ai, x_, _, _) (G0 : G) => Map.add x_ (ctxv_T Ai) G0) G0 T_x_t_y_list) e0 A ->
   NoDup (map (fun '(_, _, _, y) => y) T_x_t_y_list) ->
-  (* needed? *)
+  NoDup (map (fun '(_, x, _, _) => x) T_x_t_y_list) ->
   fresh_vars_e (map (fun '(_, _, _, y) => y) T_x_t_y_list) e0 ->
+  disjoint (map (fun '(_, _, _, y) => y) T_x_t_y_list) (map (fun '(_, x, _, _) => x) T_x_t_y_list) ->
   typ_e (fold_right (fun '(Ai, _, _, y) (G0 : G) => Map.add y (ctxv_T Ai) G0) G0 T_x_t_y_list)
     (e_var_subst e0 (map (fun '(_, x_, _, y_) => (x_, y_)) T_x_t_y_list)) A.
 Proof.
   intros.
   generalize dependent G0.
+  generalize dependent e0.
   induction T_x_t_y_list; intros.
   - easy.
   - destruct a as (((?T_,?x_),?t_),?y).
     unfold e_var_subst.
-    simpl.
+    simpl in *.
     inv H0.
-    apply subst_lemma_one_alt.
-    + replace (fold_right (fun '(x', y') (e' : e) => e_var_subst_one e' x' y') e0 (map (fun '(_, x_, _, y_) => (x_, y_)) T_x_t_y_list))
-        with (e_var_subst e0 (map (fun '(_, x_, _, y_) => (x_, y_)) T_x_t_y_list)) by auto.
-      simpl in H, H1.
-      apply fresh_monotone_e in H1.
+    inv H1.
+    pose proof fresh_first_e _ _ _ H2.
+    pose proof fresh_monotone_e _ _ _ H2.
+    epose proof disjoint_monotone _ _ _ _ H3.
+    assert (~ In x_ (map (fun '(_, y) => y) (map (fun '(Ai, _, _, y1) => (Ai, y1)) T_x_t_y_list))).
+    { intro.
+      apply (H3 x_).
+      - right.
+        rewrite map_map in H9.
+        replace (map (fun '(_, _, _, y1) => y1) T_x_t_y_list)
+          with
+            (map (fun x0 : T * x * t * x => let '(_, y) := let '(Ai, _, _, y1) := x0 in (Ai, y1) in y) T_x_t_y_list).
+        apply H9.
+        apply map_eq.
+        now intros (((?, ?), ?), ?).
+      - now left.
+    }
+    replace (Map.add x_ (ctxv_T T_) (fold_right (fun '(Ai, x_, _, _) (G0 : G) => Map.add x_ (ctxv_T Ai) G0) G0 T_x_t_y_list))
+      with (fold_right (fun '(Ai, x_, _, _) (G0 : G) => Map.add x_ (ctxv_T Ai) G0) (Map.add x_ (ctxv_T T_) G0) T_x_t_y_list)
+      in H.
+    pose proof IHT_x_t_y_list H7 H8 H4 _ H1 _ H as IH.
+    replace (fold_right (fun '(Ai, _, _, y) (G0 : G) => Map.add y (ctxv_T Ai) G0) (Map.add x_ (ctxv_T T_) G0) T_x_t_y_list)
+      with (Map.add x_ (ctxv_T T_) (fold_right (fun '(Ai, _, _, y) (G0 : G) => Map.add y (ctxv_T Ai) G0) G0 T_x_t_y_list))
+      in IH.
+    assert (fresh_vars_e [y] (e_var_subst e0 (map (fun '(_, x_, _, y_) => (x_, y_)) T_x_t_y_list))).
+    {
+      assert (map snd (map (fun '(_, x_0, _, y_) => (x_0, y_)) T_x_t_y_list) = map (fun '(_, _, _, y) => y) T_x_t_y_list).
+      {
+        rewrite map_map.
+        apply map_eq.
+        now intros (((?, ?), ?), ?).
+      }
+      apply fresh_var_subst; try rewrite H10; auto.
+    }
+    now apply (subst_lemma_one _ _ _ _ _ _ IH H10).
+
+    (* resolving those replaces from earlier *)
+    {
+      epose proof fold_add_comm G0 x_ T_ (map (fun '(Ai, _, _, y1) => (Ai, y1)) T_x_t_y_list) H9.
+      rewrite 2 fold_map1.
+      Fail apply H10.
+      (* why? *)
       admit.
-
-    + apply fresh_vars_first in H1.
-      apply fresh_subst_NoDup; eauto.
-      intro.
-      apply H4.
-      rewrite map_map in H0.
-      apply in_map_iff in H0.
-      destruct H0 as ((((?,?),?), ?), (?, ?)); subst.
-      apply in_map_iff.
-      eexists.
-      split; now eauto.
+    }
+    {
+      epose proof fold_add_comm G0 x_ T_ (map (fun '(Ai, _, _, y1) => (Ai, y1)) T_x_t_y_list) H9.
+      rewrite 2 fold_map2.
+      Fail rewrite <- H10.
+      (* why? *)
+      admit.
+    }
 Admitted.
-
 
 Lemma type_preservation : forall (Flist : list F) (G5 : G) (s5 : s),
   G_vdash_s G5 s5 ->
@@ -859,21 +630,21 @@ Proof.
     pose proof utils.in_split F_list F'_list fn_def .
     rewrite app_nil_r in *.
     pose proof Forall_forall (typ_F G5) (F_list ++ [fn_def] ++ F'_list) as (? & _).
-    pose proof H1 F_well_typed fn_def H0 as fn_typed.
+    pose proof H2 F_well_typed fn_def H1 as fn_typed.
     inv fn_typed.
     inv e0_type.
     destruct H as ((?, ?), ?).
     assert (e_T_list = map (fun '(T_, _, t_, _) => (e_t t_, T_)) T_x_t_y_list).
     {
-      rewrite H5 in H9.
-      inv H9.
+      (* inv H11. *)
       eapply map_split'.
       - replace (map fst e_T_list) with (map (fun pat_ : e * T => let (e_, _) := pat_ in e_) e_T_list) by easy.
-        rewrite H3.
+        rewrite H4.
         apply map_ext.
         easy.
       - replace (map snd e_T_list) with (map (fun pat_ : e * T => let (_, T_) := pat_ in T_) e_T_list) by easy.
-        rewrite <- H10.
+        rewrite H7 in H11.
+        inv H11.
         rewrite map_map.
         apply map_ext.
         intros.
@@ -884,25 +655,23 @@ Proof.
     + eapply fresh_subG; eauto.
     + rewrite <- fold_map.
       apply fresh_consistent; eauto.
-      (* some slightly silly reshuffling *)
       intros.
-      apply in_map_iff in H10.
-      destruct H10 as (Txty, (?, ?)).
+      apply in_map_iff in H12.
+      destruct H12 as (Txty, (?, ?)).
       apply H6.
-      rewrite H7.
+      inv H12.
       rewrite map_map.
       apply in_map_iff.
       exists Txty.
       split; auto.
       destruct Txty as (((?, ?), ?), ?).
-      now inv H10.
+      now inv H15.
 
-(* here the ABS paper appeals to type preservation under substitutions, but that seems like overkill*)
-    + rewrite H5 in H9.
-      inv H9.
+    + rewrite H7 in H11.
+      inv H11.
       apply subst_lemma; auto.
-      rewrite <- fold_map_reshuffle.
-      apply H8.
+      * rewrite <- fold_map_reshuffle; eauto.
+      * rewrite map_xs in H10.
+        apply H10.
 Qed.
-
 End FunctionalMetatheory.
