theories/utils.v
@@ -1,4 +1,5 @@
 From Coq Require Import List
+  FSets.FMapFacts
   Lia.
 
 Import ListNotations.
@@ -47,7 +48,17 @@ Section ListLemmas.
         rewrite (IHl l2); auto.
   Qed.
 
-  (* extremely ad-hoc*)
+  Lemma map_xs {Z W: Type}: forall (T_x_t_y_list: list (X*Y*Z*W)),
+      map (fun pat_ : X * Y => let (_, x_) := pat_ in x_) (map (fun '(T_, x_, _, _) => (T_, x_)) T_x_t_y_list) =
+        map (fun '(_, x, _, _) => x) T_x_t_y_list.
+  Proof.
+    induction T_x_t_y_list.
+    - easy.
+    - destruct a as (((?, ?), ?), ?).
+      simpl.
+      now rewrite IHT_x_t_y_list.
+  Qed.
+
   Lemma map_split' {Z Z' W: Type}: forall (l: list (Z'*X)) (l2: list (X*Y*Z*W)) (f: Z -> Z'),
       map fst l = map (fun '(_, _, z, _) => f z) l2 ->
       map snd l = map (fun '(x, _, _, _) => x) l2 ->
@@ -209,6 +220,39 @@ Section ListLemmas.
     now rewrite IHl.
   Qed.
 
+  Lemma fold_map1 {A Z W: Type}: forall (f: W -> X -> A -> A) (l: list (X*Y*Z*W)) a0,
+      fold_right (fun '(z, _, _, w) a => f w z a) a0 l =
+        fold_right (fun '(z, w) a => f z w a) a0
+          (map (fun '(z, _, _, w) => (w, z)) l).
+  Proof.
+    induction l; intros; eauto.
+    destruct a as [[[? ?] ?] ?].
+    simpl.
+    now rewrite IHl.
+  Qed.
+
+  Lemma fold_map2 {A Z W: Type}: forall (f: Y -> X -> A -> A) (l: list (X*Y*Z*W)) a0,
+      fold_right (fun '(z, w, _, _) a => f w z a) a0 l =
+        fold_right (fun '(z, w) a => f z w a) a0
+          (map (fun '(z, w, _, _) => (w, z)) l).
+  Proof.
+    induction l; intros; eauto.
+    destruct a as [[[? ?] ?] ?].
+    simpl.
+    now rewrite IHl.
+  Qed.
+
+  Lemma fold_map3 {A Z W: Type}: forall (f: W -> Y -> A -> A) (l: list (X*Y*Z*W)) a0,
+      fold_right (fun '(_, z, _, w) a => f w z a) a0 l =
+        fold_right (fun '(z, w) a => f z w a) a0
+          (map (fun '(_, z, _, w) => (w, z)) l).
+  Proof.
+    induction l; intros; eauto.
+    destruct a as [[[? ?] ?] ?].
+    simpl.
+    now rewrite IHl.
+  Qed.
+
   Lemma combine_map: forall (l: list (X*Y)),
       combine (map fst l) (map snd l) = l.
   Proof.
@@ -293,3 +337,352 @@ Section ListLemmas.
   Qed.
 
 End ListLemmas.
+
+Require Import FMapList OrderedTypeEx.
+From ABS Require Import abs_defs.
+From Equations Require Import Equations.
+
+Module MapFacts := FSets.FMapFacts.Facts Map.
+
+
+(* some slightly ad-hoc equalities *)
+Lemma subst_fst_commute: forall x0 x1 e_T_list,
+  map (fun x : e * T => let (e_, _) := let '(e_, T_) := x in (e_var_subst_one e_ x0 x1, T_) in e_) e_T_list =
+  (fix e_list_subst_one (es : list e) (x_ y_ : x) {struct es} : list e :=
+     match es with
+     | [] => fun _ _ : x => []
+     | e :: l => fun x_0 y_0 : x => e_var_subst_one e x_0 y_0 :: e_list_subst_one l x_0 y_0
+     end x_ y_) (map (fun pat_ : e * T => let (e_, _) := pat_ in e_) e_T_list) x0 x1.
+Proof.
+  induction e_T_list; auto.
+  destruct a.
+  simpl.
+  rewrite <- IHe_T_list.
+  reflexivity.
+Qed.
+
+Lemma subst_snd_commutes: forall x0 s e_T_list,
+  map (fun pat_ : e * T => let (_, T_) := pat_ in T_)
+    (map (fun pat_ : e * T => let (e_, T_) := pat_ in (e_var_subst_one e_ x0 s, T_)) e_T_list) =
+    map (fun pat_ : e * T => let (_, T_) := pat_ in T_) e_T_list.
+Proof.
+  intros.
+  induction e_T_list; auto.
+  destruct a;cbn in *.
+  now rewrite IHe_T_list.
+Qed.
+
+(* Characterizing substitution *)
+
+Lemma subst_term: forall t sub,
+  e_var_subst (e_t t) sub = (e_t t).
+Proof.
+  induction sub.
+  - trivial.
+  - destruct a.
+    simpl.
+    rewrite IHsub.
+    now simp e_var_subst_one.
+Qed.
+
+Definition replace_var (x0:x) (sub:list(x*x)) :=
+ fold_right (fun '(x_, y_) x0 => if (eq_x x0 x_) then y_ else x0) x0 sub.
+
+Lemma subst_var: forall x0 sub,
+  e_var_subst (e_var x0) sub = e_var (replace_var x0 sub).
+Proof.
+  induction sub.
+  - trivial.
+  - destruct a; simpl.
+    rewrite IHsub.
+    simp e_var_subst_one.
+    destruct (eq_x (replace_var x0 sub)); subst; eauto.
+Qed.
+
+Lemma e_list_subst_map: forall x0 y0 e_list,
+  e_list_subst_one e_list x0 y0 = map (fun e_ => e_var_subst_one e_ x0 y0) e_list.
+Proof.
+  induction e_list; [easy|];
+  destruct a;
+    simpl;
+    now rewrite IHe_list.
+Qed.
+
+Lemma subst_fn: forall fn0 sub e_list,
+  e_var_subst (e_fn_call fn0 e_list) sub = (e_fn_call fn0 (map (fun e' => e_var_subst e' sub) e_list)).
+Proof.
+  induction sub; intros.
+  - simpl.
+    now rewrite map_id.
+  - destruct a.
+    simpl.
+    rewrite IHsub.
+    simp e_var_subst_one.
+    now rewrite e_list_subst_map, map_map.
+Qed.
+
+Lemma e_list_subst: forall el x0 y0,
+  e_list_subst_one el x0 y0 = map (fun e => e_var_subst_one e x0 y0) el.
+Proof.
+  induction el; intros.
+  - trivial.
+  - simpl.
+    now rewrite IHel.
+Qed.
+
+Lemma e_list_fresh: forall e0 ys el,
+  fresh_vars_el ys el ->
+  In e0 el ->
+  fresh_vars_e ys e0.
+Proof.
+  induction el.
+  - easy.
+  - simpl; intros.
+    destruct H0; subst.
+    + now destruct H.
+    + destruct H.
+      apply IHel; eauto.
+Qed.
+
+(* Properties of fresh_e*)
+Lemma fresh_first_e: forall e0 y ys,
+  fresh_vars_e (y::ys) e0 -> fresh_vars_e [y] e0.
+Proof.
+  induction e0 using e_ott_ind
+    with (P_list_e := fun e_list =>
+                        forall e0 y ys,
+                        In e0 e_list ->
+                        fresh_vars_e (y::ys) e0 -> fresh_vars_e [y] e0);
+     intros; try easy.
+  - simp fresh_vars_e in *.
+    intro.
+    inv H0.
+    + apply H.
+    now left.
+    + inv H1.
+  - simp fresh_vars_e in *.
+    induction e_list.
+    + easy.
+    + inv H.
+      split.
+      * eapply IHe0; eauto.
+        now left.
+      * eapply IHe_list; eauto.
+        intros; eapply IHe0; eauto.
+        now right.
+  - inv H.
+    + eapply IHe0; eauto.
+    + eapply IHe1; eauto.
+Qed.
+
+Lemma fresh_monotone_e: forall e0 y ys,
+  fresh_vars_e (y::ys) e0 -> fresh_vars_e ys e0.
+Proof.
+  induction e0 using e_ott_ind
+    with (P_list_e := fun e_list =>
+                        forall e0 y ys,
+                        In e0 e_list ->
+                        fresh_vars_e (y::ys) e0 -> fresh_vars_e ys e0);
+     intros; try easy.
+  - simp fresh_vars_e in *.
+    intro.
+    apply H.
+    right.
+    assumption.
+  - simp fresh_vars_e in *.
+    induction e_list.
+    + easy.
+    + inv H.
+      split.
+      * eapply IHe0; eauto.
+        now left.
+      * apply IHe_list; eauto.
+        intros; eapply IHe0; eauto.
+        now right.
+  - inv H.
+    + eapply IHe0; eauto.
+    + eapply IHe1; eauto.
+Qed.
+
+Lemma fresh_first_el: forall el y ys,
+    fresh_vars_el (y::ys) el -> fresh_vars_el [y] el.
+Proof.
+  induction el; intros.
+  - now inv H.
+  - inv H.
+    split.
+    + now apply fresh_first_e in H0.
+    + eapply IHel; eauto.
+Qed.
+
+Lemma fresh_monotone_el: forall el y ys,
+  fresh_vars_el (y::ys) el -> fresh_vars_el ys el.
+Proof.
+  induction el; intros.
+  - now inv H.
+  - inv H.
+    split.
+    + now apply fresh_monotone_e in H0.
+    + eapply IHel; eauto.
+Qed.
+
+Lemma fresh_var_subst: forall e0 y sub,
+  fresh_vars_e (map snd sub) e0 ->
+  fresh_vars_e [y] e0 ->
+  ~ In y (map snd sub) ->
+  fresh_vars_e [y] (e_var_subst e0 sub).
+Proof.
+  intros.
+  generalize dependent y.
+  generalize dependent e0.
+  induction e0 using e_ott_ind
+    with
+    (P_list_e := fun e_list => forall y,
+                     fresh_vars_el (map snd sub) e_list ->
+                     fresh_vars_el [y] e_list ->
+                     ~ In y (map snd sub) ->
+                     fresh_vars_el [y] (map (fun e' => e_var_subst e' sub) e_list))
+  ; intros; auto.
+  - rewrite subst_term.
+    now simp e_var_subst_one.
+  - induction sub; auto.
+    destruct a as (?x_, ?y); simpl.
+    rewrite subst_var.
+    simp e_var_subst_one.
+    destruct (eq_x (replace_var x5 sub) x_).
+    + simp fresh_vars_e.
+      intro.
+      apply H1.
+      left.
+      now inv H2.
+    + rewrite <- subst_var.
+      apply Decidable.not_or in H1.
+      destruct H1.
+      apply fresh_monotone_e in H.
+      eapply IHsub; auto.
+  - rewrite subst_fn.
+    simp fresh_vars_e in *.
+  - destruct H,H0.
+    split.
+    + apply IHe0; auto.
+    + apply IHe1; eauto.
+Qed.
+
+Fact disjoint_empty{A:Type}: @disjoint A [] [].
+Proof. easy. Qed.
+
+Lemma disjoint_monotone {A:Type}: forall (l1 l2: list A) a1 a2,
+  disjoint (a1::l1) (a2::l2) -> disjoint l1 l2.
+Proof.
+  intros.
+  intros ? ? ?.
+    specialize (H a).
+    apply H; now right.
+Qed.
+
+Section MapLemmas.
+
+  Lemma map_neq_none_is_some{elt:Type}: forall m x,
+      Map.find x m <> None ->
+      exists y, Map.find (elt:=elt) x m = Some y.
+  Proof.
+    intros.
+    destruct (MapFacts.In_dec m x).
+    - inv i.
+      exists x0.
+      apply Map.find_1.
+      apply H0.
+    - apply MapFacts.not_find_in_iff in n.
+      rewrite n in H.
+      contradiction.
+  Qed.
+
+  Lemma fold_map_reshuffle: forall (l: list (T*x*t*x)) G0,
+      (fold_right (fun (ax : x * T) (G' : G) => Map.add (fst ax) (ctxv_T (snd ax)) G') G0
+         (map (fun pat_ : T * x => let (T_, x_) := pat_ in (x_, T_)) (map (fun '(T_0, x_, _, _) => (T_0, x_)) l)))
+      = (fold_right (fun '(T1, x_, _, _) (G' : G) => Map.add x_ (ctxv_T T1) G') G0 l).
+  Proof.
+    induction l;intros;auto.
+    destruct a as (((?T_ & ?x_) & ?t_) & ?y).
+    simpl.
+    rewrite IHl.
+    reflexivity.
+  Qed.
+
+  Lemma map_add_comm{E:Type}: forall m key key' elt elt',
+      key <> key' -> Map.Equal (Map.add (elt:=E) key elt (Map.add key' elt' m)) (Map.add key' elt' (Map.add key elt m)).
+  Proof.
+    intros.
+    intro.
+    destruct (Map.find y m) eqn:?.
+    - destruct (eq_x y key), (eq_x y key'); subst;
+        erewrite 2 Map.find_1; eauto;
+        (* this should just be "eauto with map", but I can't seem to import the hint database *)
+        try (apply Map.add_2; eauto; now apply Map.add_1);
+        try (now apply Map.add_1; eauto);
+        try (repeat (apply Map.add_2; eauto); now apply Map.find_2; eauto).
+    - destruct (eq_x y key), (eq_x y key'); subst.
+      + contradiction.
+      + erewrite 2 Map.find_1; eauto.
+        * apply Map.add_2; eauto.
+          now apply Map.add_1.
+        * now apply Map.add_1.
+      + erewrite 2 Map.find_1; eauto.
+        * now apply Map.add_1.
+        * apply Map.add_2; eauto.
+          now apply Map.add_1.
+
+      (* there has to be a cleaner way to do this case?? *)
+      + replace (Map.find (elt:=E) y (Map.add key elt (Map.add key' elt' m))) with (@None E).
+        replace (Map.find (elt:=E) y (Map.add key' elt' (Map.add key elt m))) with (@None E).
+        reflexivity.
+        * symmetry.
+          apply MapFacts.not_find_in_iff in Heqo.
+          apply MapFacts.not_find_in_iff.
+          intro.
+          apply Heqo.
+          inv H0.
+          exists x.
+          apply Map.add_3  with (x:= key) (e':=elt); auto.
+          apply Map.add_3 with (x:=key') (e':=elt'); auto.
+        * symmetry.
+          apply MapFacts.not_find_in_iff in Heqo.
+          apply MapFacts.not_find_in_iff.
+          intro.
+          inv H0.
+          apply Heqo.
+          exists x.
+          apply Map.add_3 with (x:=key') (e':=elt'); auto.
+          apply Map.add_3  with (x:= key) (e':=elt); auto.
+  Qed.
+
+  Lemma fold_not_in: forall G0 y (T_x_t_y_list: list (T*x*t*x)),
+      ~ Map.In y G0 ->
+      ~ In y (map (fun '(_, _, _, y') => y') T_x_t_y_list) ->
+      ~ Map.In y (fold_right (fun '(T_, _, _, y) (G0 : G) => Map.add y (ctxv_T T_) G0) G0 T_x_t_y_list).
+  Proof.
+    induction T_x_t_y_list as [ | (((?T_, ?x_), ?t_), ?y) T_x_t_y_list IH ]; [easy|].
+    simpl; intros ? ? ?.
+    destruct (eq_x y y0); subst.
+    - apply H0.
+      now left.
+    - apply MapFacts.add_in_iff in H1.
+      inv H1.
+      + apply H0.
+        now left.
+      + apply IH; eauto.
+  Qed.
+
+  Lemma fold_add_comm: forall G0 y T_ (upd: list (T*x)),
+      ~ In y (map (fun '(_, y) => y) upd) ->
+      Map.Equal (Map.add y (ctxv_T T_) (fold_right (fun '(T_, y) G0 => Map.add y (ctxv_T T_) G0) G0 upd))
+        (fold_right (fun '(T_, y) G0 => Map.add y (ctxv_T T_) G0) (Map.add y (ctxv_T T_) G0) upd).
+  Proof.
+    induction upd; intros.
+    - easy.
+    - destruct a; simpl in *.
+      apply Decidable.not_or in H.
+      destruct H.
+      now rewrite map_add_comm, IHupd; auto.
+  Qed.
+End MapLemmas.
